Monad_Play Around/DNFP/Dutch_National_Flag_Monad_Definitions_Lemmas.thy
@@ -20,7 +20,7 @@ lemma value_must_be_two : "\<lbrakk>xs e ! i e  > 0 ; xs e! i e > 1 ; i e < leng
 lemma value_must_be_one_aux : "\<lbrakk>\<not>xs e ! i e  > 1 ; \<not>xs e! i e < 1 ; i e < length (xs e) ; set(xs e) \<subseteq> {0,1,2}\<rbrakk> \<Longrightarrow> xs e ! i e = 1"
   by linarith
 
-section\<open>Inc_lowbound - proof\<close>
+section\<open>Inc lowbound - proof\<close>
 
 text\<open>Inc lowbound will keep relationship between variables and inc i and low\<close>
 lemma inc_lowbound_spec: "spec (inc_lowbound_pre e) inc_lowbound (GG (inc_lowbound_post e))"
@@ -118,7 +118,7 @@ lemma inc_lowbound_spec: "spec (inc_lowbound_pre e) inc_lowbound (GG (inc_lowbou
    apply(intro get_rule; intro allI)
   by(simp add: spec_def put_def get_state_def put_state_def low_Env_def)
 
-subsection\<open>Invariants - inc_lowbound\<close>
+subsection\<open>Invariants - inc lowbound\<close>
 lemma inc_lowbound_invariantRed: "spec inc_lowbound_inv1_aux inc_lowbound (GG inc_lowbound_inv1)"
   unfolding inc_lowbound_inv1_aux_def inc_lowbound_inv1_def loop_update_action_pre_def  GG_def low_invariant_is_0_Env_def dnfp_variables_invariants_def
   apply(simp_all add: inc_lowbound_def)
@@ -193,7 +193,7 @@ text\<open>All invariants are preserved\<close>
 lemma inc_lowbound_invariants: "spec inc_lowbound_inv_pre  inc_lowbound (GG inc_lowbound_inv)"
   by (smt GG_def case_prodD case_prodI2 inc_lowbound_inv1_aux_def inc_lowbound_inv2_aux_def inc_lowbound_inv3_aux_def inc_lowbound_inv_def inc_lowbound_inv_pre_def inc_lowbound_invariantBlue inc_lowbound_invariantRed inc_lowbound_invariantWhite spec_def)
 
-section\<open>Dec_highbound proof\<close>                                          
+section\<open>Dec highbound proof\<close>                                          
 lemma dec_highbound_spec: "spec (dec_highbound_pre e) dec_highbound (GG (dec_highbound_post e))"
   unfolding dec_highbound_pre_def dnfp_variables_invariants_def dnfp_post_def loop_update_action_pre_def GG_def dec_highbound_post_def loop_update_action_post_def
   apply(simp_all add: dec_highbound_def)
@@ -313,7 +313,7 @@ lemma dec_highbound_invariantBlue: "spec dec_highbound_inv3_aux dec_highbound (G
 lemma dec_highbound_invariants: "spec dec_highbound_inv_aux dec_highbound (GG dec_highbound_inv)"
   by (smt GG_def case_prodD case_prodI2 dec_highbound_inv1_aux_def dec_highbound_inv2_aux_def dec_highbound_inv3_aux_def dec_highbound_inv_aux_def dec_highbound_inv_def dec_highbound_invariantBlue dec_highbound_invariantRed dec_highbound_invariantWhite spec_def)
 
-section\<open>Inc_index proof\<close>
+section\<open>Inc index proof\<close>
 lemma inc_index_spec: "spec (inc_index_pre e) inc_index (GG (inc_index_post e))"
   unfolding inc_index_pre_def dnfp_variables_invariants_def dnfp_post_def loop_update_action_pre_def GG_def inc_index_post_def loop_update_action_post_def
   apply(simp_all add: inc_index_def)
@@ -323,7 +323,7 @@ lemma inc_index_spec: "spec (inc_index_pre e) inc_index (GG (inc_index_post e))"
    apply linarith
   by linarith
 
-subsection\<open>Invariants - inc_index\<close>
+subsection\<open>Invariants - inc index\<close>
 lemma inc_index_invariantRed: "spec inc_index_inv1_aux inc_index (GG inc_index_inv1)"
   unfolding inc_index_inv1_aux_def inc_index_inv1_def dnfp_variables_invariants_def loop_update_action_pre_def  GG_def low_invariant_is_0_Env_def
   apply(simp_all add: inc_index_def)
@@ -476,7 +476,7 @@ lemma loop_update_action_spec: "spec (loop_update_action_pre_aux e) loop_update_
   apply (simp add: diff_le_mono2)
   by (simp add: Suc_diff_Suc)
 
-subsection\<open>Invariants - Loop_update_action \<close>                                                       
+subsection\<open>Invariants - Loop update action \<close>                                                       
 lemma loop_update_action_invariantRed: "spec loop_update_action_inv1_aux loop_update_action (GG loop_update_action_inv1)"
    unfolding loop_update_action_inv1_aux_def loop_update_action_inv1_def dnfp_variables_invariants_def  loop_update_action_pre_def  GG_def low_invariant_is_0_Env_def
   apply(simp add: loop_update_action_def)
